bounding permissions by 1.0 behind the scenes

pulse/ulib/experimental/Steel.PCM.HigherReference.fst
@@ -22,6 +22,7 @@ open FStar.Ghost
 open FStar.Real
 open Steel.PCM
 open Steel.PCM.FractionalPermission
+module Atomic = Steel.PCM.Effect.Atomic
 
 let fractional (a:Type u#1) = option (a & perm)
 #push-options "--query_stats"
@@ -53,36 +54,103 @@ let pcm_frac #a : pcm (fractional a) = {
 module Mem = Steel.PCM.Memory
 
 let ref a = Mem.ref (fractional a) pcm_frac
-let pts_to #a r p v = Mem.pts_to r (Some (Ghost.reveal v, p))
-
-let alloc #a x =
-  let v = Some (x, full_perm) in
-  assert (Steel.PCM.composable pcm_frac v None);
-  assert (compatible pcm_frac v v);
-  Steel.PCM.Effect.alloc v
-
-assume
-val sl_assert (p:slprop)
-  : SteelT unit p (fun _ -> p)
+let perm_ok p : prop = (p.v <=. 1.0R == true) /\ True
+let pts_to_raw (#a:Type) (r:ref a) (p:perm) (v:erased a) = Mem.pts_to r (Some (Ghost.reveal v, p))
+let pts_to #a r p v = pts_to_raw r p v `star` pure (perm_ok p)
 
 assume
 val sl_admit (#a:_) (#p:_) (q:a -> slprop)
   : SteelT a p q
 
 assume
+val sl_admit_atomic (#a:_) (#uses:_) (#p:_) (q:a -> slprop)
+  : SteelAtomic a uses unobservable p q
+
+assume
+val sl_assert (p:slprop)
+  : SteelT unit p (fun _ -> p)
+
+assume
 val sl_return (#a:_) (p:a -> slprop) (x:a)
   : SteelT a (p x) p
 
 assume
-val drop (p:slprop)
+val elim_pure (#uses:_) (p:prop)
+  : SteelAtomic (_:unit{p}) uses unobservable
+                (pure p)
+                (fun _ -> emp)
+
+let drop (p:slprop)
   : SteelT unit p (fun _ -> emp)
+  = lift_atomic_to_steelT (fun _ ->
+    Atomic.change_slprop _ _ (fun m -> emp_unit p; affine_star p emp m))
+
+let comm (#opened_invariants:inames)
+         (#p #q:slprop) (_:unit)
+  : SteelAtomic unit opened_invariants unobservable
+                (p `star` q)
+                (fun x -> q `star` p)
+  = Atomic.change_slprop _ _ (fun m -> Mem.star_commutative p q)
+
+let intro_perm_ok #uses (p:perm{perm_ok p}) (q:slprop)
+  : SteelAtomic unit uses unobservable
+                q
+                (fun _ -> q `star` pure (perm_ok p))
+  = Atomic.change_slprop _ _
+    (fun m -> emp_unit q; pure_star_interp q (perm_ok p) m)
+
+let elim_perm_ok #uses (p:perm)
+  : SteelAtomic (q:perm{perm_ok q /\ q == p}) uses unobservable
+                (pure (perm_ok p))
+                (fun _ -> emp)
+  = let _ = elim_pure (perm_ok p) in
+    Atomic.return_atomic p
+
+let intro_pts_to (p:perm{perm_ok p}) #a #uses (#v:erased a) (r:ref a) (_:unit)
+  : SteelAtomic unit uses unobservable
+                (pts_to_raw r p v)
+                (fun _ -> pts_to r p v)
+  = intro_perm_ok p _
+
+let intro_pure (#a:_) (#p:a -> slprop) (q:perm { perm_ok q }) (x:a)
+  : SteelT a (p x) (fun y -> p y `star` pure (perm_ok q))
+  = Atomic.lift_atomic_to_steelT (fun _ -> intro_perm_ok q _);
+    sl_return _ x
+
+let drop_l_atomic #uses (#p #q:slprop)  ()
+  : SteelAtomic unit uses unobservable (p `star` q) (fun _ -> q)
+  = Atomic.change_slprop _ _ (affine_star p q)
+
+let elim_pure_atomic #uses  (#p:perm -> slprop) (q:perm)
+  : SteelAtomic (q':perm{perm_ok q' /\ q == q'}) uses unobservable
+                (p q `star` pure (perm_ok q))
+                (fun q' -> p q')
+  = comm();
+    let q' = Atomic.frame _ (fun _ -> elim_perm_ok q) in
+    h_assert_atomic (emp `star` p q);
+    drop_l_atomic ();
+    Atomic.return_atomic q'
+
+let elim_perm_ok_star (#p:slprop) (q:perm)
+  : SteelT (_:unit{perm_ok q}) (p `star` pure (perm_ok q))
+           (fun _ -> p)
+  = let _ = Atomic.lift_atomic_to_steelT (fun () -> elim_pure_atomic #Set.empty #(fun _ -> p) q) in
+    sl_return _ ()
+
+let alloc #a x =
+  let v = Some (x, full_perm) in
+  assert (Steel.PCM.composable pcm_frac v None);
+  assert (compatible pcm_frac v v);
+  let x = Steel.PCM.Effect.alloc v in
+  intro_pure full_perm x
 
 let read (#a:Type) (#p:perm) (#v:erased a) (r:ref a)
   : SteelT a (pts_to r p v) (fun x -> pts_to r p x)
   = let v1 : erased (fractional a) = Ghost.hide (Some (Ghost.reveal v, p)) in
+    elim_perm_ok_star p;
     let v2 = Steel.PCM.Effect.read r v1 in
     let Some (x, _) = v2 in
-    sl_return #a (fun x -> pts_to r p x) x
+    intro_pure p x
 
 let read_refine (#a:Type) (#p:perm) (q:a -> slprop) (r:ref a)
   : SteelT a (h_exists (fun (v:a) -> pts_to r p v `star` q v))
@@ -93,38 +161,70 @@ let write (#a:Type) (#v:erased a) (r:ref a) (x:a)
   : SteelT unit (pts_to r full_perm v) (fun _ -> pts_to r full_perm x)
   = let v_old : erased (fractional a) = Ghost.hide (Some (Ghost.reveal v, full_perm)) in
     let v_new : fractional a = Some (x, full_perm) in
-    Steel.PCM.Effect.write r v_old v_new
+    elim_perm_ok_star full_perm;
+    Steel.PCM.Effect.write r v_old v_new;
+    intro_pure full_perm ()
 
 let free (#a:Type) (#v:erased a) (r:ref a)
   : SteelT unit (pts_to r full_perm v) (fun _ -> emp)
   = let v_old : erased (fractional a) = Ghost.hide (Some (Ghost.reveal v, full_perm)) in
+    elim_perm_ok_star full_perm;
     Steel.PCM.Effect.free r v_old;
     drop _
 
 (* move these to Mem *)
-let mem_share_atomic (#a:Type) (#uses:_) (#p:perm) (r:ref a)
-                     (v0:erased a)
-  : action_except unit uses (pts_to r p v0)
-                            (fun _ -> pts_to r (half_perm p) v0 `star` pts_to r (half_perm p) v0)
-  = assume (p.v <=. 1.0R);
-    let v = Ghost.hide (Some (Ghost.reveal v0, half_perm p)) in
+let mem_share_atomic_raw (#a:Type) (#uses:_) (#p:perm{perm_ok p}) (r:ref a)
+                         (v0:erased a)
+  : action_except unit uses (pts_to_raw r p v0)
+                            (fun _ -> pts_to_raw r (half_perm p) v0 `star` pts_to_raw r (half_perm p) v0)
+  = let v = Ghost.hide (Some (Ghost.reveal v0, half_perm p)) in
     Mem.split_action uses r v v
 
-let mem_gather_atomic (#a:Type) (#uses:_) (#p0 #p1:perm) (r:ref a) (v0:erased a) (v1:erased a)
-  : action_except (_:unit{v0 == v1}) uses
-                  (pts_to r p0 v0 `star` pts_to r p1 v1)
-                  (fun _ -> pts_to r (sum_perm p0 p1) v0)
-  = let v0 = Ghost.hide (Some (Ghost.reveal v0, p0)) in
-    let v1 = Ghost.hide (Some (Ghost.reveal v1, p1)) in
-    Mem.gather_action uses r v0 v1
+let share_atomic_raw #a #uses (#p:perm) (r:ref a{perm_ok p}) (v0:erased a)
+  : SteelAtomic unit uses unobservable
+                (pts_to_raw r p v0)
+                (fun _ -> pts_to_raw r (half_perm p) v0 `star` pts_to_raw r (half_perm p) v0)
+  = as_atomic_action (mem_share_atomic_raw r v0)
 
 let share (#a:Type) #uses (#p:perm) (#v:erased a) (r:ref a)
   : SteelAtomic unit uses unobservable
                (pts_to r p v)
                (fun _ -> pts_to r (half_perm p) v `star` pts_to r (half_perm p) v)
-  = as_atomic_action (mem_share_atomic r v)
+  = let p = elim_pure_atomic #_ #(fun q -> pts_to_raw r q v) p in
+    share_atomic_raw r v;
+    h_assert_atomic (pts_to_raw r (half_perm p) v `star` pts_to_raw r (half_perm p) v);
+    Steel.PCM.Effect.Atomic.frame _
+                                  (intro_pts_to (half_perm p) r);
+    h_assert_atomic (pts_to r (half_perm p) v `star` pts_to_raw r (half_perm p) v);
+    comm ();
+    h_assert_atomic (pts_to_raw r (half_perm p) v `star` pts_to r (half_perm p) v);
+    Steel.PCM.Effect.Atomic.frame #unit #uses #unobservable
+                                  #(pts_to_raw r (half_perm p) v)
+                                  #(fun _ -> pts_to r (half_perm p) v)
+                                  (pts_to r (half_perm p) v)
+                                  (intro_pts_to (half_perm p) r)
+
+let mem_gather_atomic_raw (#a:Type) (#uses:_) (#p0 #p1:perm) (r:ref a) (v0:erased a) (v1:erased a)
+  : action_except (_:unit{v0==v1 /\ perm_ok (sum_perm p0 p1)}) uses
+                  (pts_to_raw r p0 v0 `star` pts_to_raw r p1 v1)
+                  (fun _ -> pts_to_raw r (sum_perm p0 p1) v0)
+  = let v0 = Ghost.hide (Some (Ghost.reveal v0, p0)) in
+    let v1 = Ghost.hide (Some (Ghost.reveal v1, p1)) in
+    Mem.gather_action uses r v0 v1
+
+let gather_atomic_raw (#a:Type) (#uses:_) (#p0 #p1:perm) (r:ref a) (v0:erased a) (v1:erased a)
+  : SteelAtomic  (_:unit{v0==v1 /\ perm_ok (sum_perm p0 p1)}) uses unobservable
+                 (pts_to_raw r p0 v0 `star` pts_to_raw r p1 v1)
+                 (fun _ -> pts_to_raw r (sum_perm p0 p1) v0)
+  = as_atomic_action (mem_gather_atomic_raw r v0 v1)
 
 let gather (#a:Type) (#uses:_) (#p0:perm) (#p1:perm) (#v0 #v1:erased a) (r:ref a)
-  = as_atomic_action (mem_gather_atomic r v0 v1)
+  = let p0 = Steel.PCM.Effect.Atomic.frame _ (fun _ -> elim_pure_atomic p0) in
+    comm();
+    let p1 = Steel.PCM.Effect.Atomic.frame _ (fun _ -> elim_pure_atomic p1) in
+    comm();
+    h_assert_atomic (pts_to_raw r p0 v0 `star` pts_to_raw r p1 v1);
+    let _ = gather_atomic_raw r v0 v1 in
+    intro_pts_to (sum_perm p0 p1) r ()
 
 let ghost_read_refine = admit()
